Upd

VRF/Spec_VRF.ml
@@ -2,11 +2,24 @@ open Prims
 type bytes = FStar_UInt8.t FStar_Seq_Base.seq
 type key = Prims.unit FStar_Endianness.lbytes
 let field: Prims.int = Spec_Curve25519.prime
-let n: Prims.int = Prims.parse_int "32"
+let n: Prims.int = Prims.parse_int "16"
 let d: Prims.int =
   Prims.parse_int
     "37095705934669439343138083508754565189542113879843219016388785533085940283555"
 type twisted_edward_point = Spec_Ed25519.ext_point
+let g_x: Prims.int =
+  Prims.parse_int
+    "15112221349535400772501151409588531511454012693041857206046113283949847762202"
+let g_y: Prims.int =
+  Prims.parse_int
+    "46316835694926478169428394003475163141307993866256225615783033603165251855960"
+let coordinality: Prims.int =
+  Prims.parse_int
+    "57896044618658097711785492504343953926856930875039260848015607506283634007912"
+let generator:
+  (Spec_Curve25519.elem* Spec_Curve25519.elem* Spec_Curve25519.elem*
+    Spec_Curve25519.elem)
+  = (g_x, g_y, (Prims.parse_int "1"), (Spec_Curve25519.fmul g_x g_y))
 let scalarMultiplication:
   twisted_edward_point -> bytes -> Spec_Ed25519.ext_point =
   fun point  -> fun k1  -> Spec_Ed25519.point_mul k1 point
@@ -25,14 +38,42 @@ let isPointOnCurve: twisted_edward_point option -> Prims.bool =
              =
              (Spec_Curve25519.fadd (Spec_Curve25519.fmul pz pz)
                 (Spec_Curve25519.fmul d (Spec_Curve25519.fmul pt pt))))
-let serializePoint: twisted_edward_point -> Prims.unit Spec_Lib.lbytes =
-  fun point  -> Spec_Ed25519.point_compress point
-let deserializePoint: bytes -> Spec_Ed25519.ext_point option =
-  fun b  -> Spec_Ed25519.point_decompress b
-let _OS2ECP: bytes -> twisted_edward_point option =
-  fun point  -> deserializePoint point
-let _ECP2OS: twisted_edward_point -> bytes =
-  fun gamma  -> serializePoint gamma
+let _OS2ECP2Points: bytes -> twisted_edward_point option =
+  fun point  ->
+    match Spec_Ed25519.recover_x
+            ((FStar_Endianness.little_endian point) mod
+               (Prims.pow2 (Prims.parse_int "255"))) true
+    with
+    | Some x ->
+        Some
+          (x,
+            (((FStar_Endianness.little_endian point) mod
+                (Prims.pow2 (Prims.parse_int "255")))
+               mod Spec_Curve25519.prime), Spec_Curve25519.one,
+            (Spec_Curve25519.fmul x
+               (((FStar_Endianness.little_endian point) mod
+                   (Prims.pow2 (Prims.parse_int "255")))
+                  mod Spec_Curve25519.prime)))
+    | uu____447 ->
+        (match Spec_Ed25519.recover_x
+                 ((FStar_Endianness.little_endian point) mod
+                    (Prims.pow2 (Prims.parse_int "255"))) false
+         with
+         | Some x ->
+             Some
+               (x,
+                 (((FStar_Endianness.little_endian point) mod
+                     (Prims.pow2 (Prims.parse_int "255")))
+                    mod Spec_Curve25519.prime), Spec_Curve25519.one,
+                 (Spec_Curve25519.fmul x
+                    (((FStar_Endianness.little_endian point) mod
+                        (Prims.pow2 (Prims.parse_int "255")))
+                       mod Spec_Curve25519.prime)))
+         | uu____487 -> None)
+let _ECP2OS: twisted_edward_point -> Prims.unit Spec_Lib.lbytes =
+  fun gamma  -> Spec_Ed25519.point_compress gamma
+let _OS2ECP: bytes -> Spec_Ed25519.ext_point option =
+  fun point  -> Spec_Ed25519.point_decompress point
 let nat_to_uint8: Prims.int -> FStar_UInt8.t =
   fun x  ->
     FStar_UInt8.uint_to_t (FStar_UInt.to_uint_t (Prims.parse_int "8") x)
@@ -43,16 +84,12 @@ let rec _helper_I2OSP:
   fun value  ->
     fun s  ->
       fun counter  ->
-        if
-          (counter + (Prims.parse_int "1")) <
-            (FStar_Seq_Base.length
-               (FStar_Seq_Base.upd s counter
-                  (nat_to_uint8 (value mod (Prims.parse_int "256")))))
+        if (counter - (Prims.parse_int "1")) >= (Prims.parse_int "0")
         then
           _helper_I2OSP (value / (Prims.parse_int "256"))
             (FStar_Seq_Base.upd s counter
                (nat_to_uint8 (value mod (Prims.parse_int "256"))))
-            (counter + (Prims.parse_int "1"))
+            (counter - (Prims.parse_int "1"))
         else
           FStar_Seq_Base.upd s counter
             (nat_to_uint8 (value mod (Prims.parse_int "256")))
@@ -67,76 +104,69 @@ let _I2OSP: Prims.nat -> Prims.int -> bytes =
         _helper_I2OSP value
           (FStar_Seq_Base.create n1
              (FStar_UInt8.uint_to_t (Prims.parse_int "0")))
-          (Prims.parse_int "0")
-let rec _helper_OS2IP: bytes -> Prims.nat -> Prims.nat -> Prims.nat =
+          (n1 - (Prims.parse_int "1"))
+let rec _helper_OS2IP: bytes -> Prims.nat -> Prims.nat -> Prims.int =
   fun s  ->
     fun counter  ->
       fun number  ->
-        if (counter + (Prims.parse_int "1")) = (FStar_Seq_Base.length s)
+        if (counter + (Prims.parse_int "1")) < (FStar_Seq_Base.length s)
         then
-          number +
-            ((Prims.pow2 (FStar_Mul.op_Star (Prims.parse_int "8") counter)) *
-               (uint8_to_int (FStar_Seq_Base.index s counter)))
-        else
           _helper_OS2IP s (counter + (Prims.parse_int "1"))
             (number +
-               ((Prims.pow2 (FStar_Mul.op_Star (Prims.parse_int "8") counter))
+               ((Prims.pow2
+                   (FStar_Mul.op_Star (Prims.parse_int "8")
+                      (((FStar_Seq_Base.length s) - counter) -
+                         (Prims.parse_int "1"))))
                   * (uint8_to_int (FStar_Seq_Base.index s counter))))
+        else
+          number +
+            ((Prims.pow2
+                (FStar_Mul.op_Star (Prims.parse_int "8")
+                   (((FStar_Seq_Base.length s) - counter) -
+                      (Prims.parse_int "1"))))
+               * (uint8_to_int (FStar_Seq_Base.index s counter)))
 let _OS2IP: bytes -> Prims.nat =
   fun s  -> _helper_OS2IP s (Prims.parse_int "0") (Prims.parse_int "0")
-
 let seqConcat s1 s2 = FStar_Seq_Base.append s1 s2
-
 let hash: bytes -> Spec_SHA2_256.bytes =
   fun input  -> Spec_SHA2_256.hash input
-(*)
 let _ECVRF_decode_proof: bytes -> (twisted_edward_point option* bytes* bytes)
   =
   fun pi  ->
-    match FStar_Seq_Properties.split pi n with
+    match FStar_Seq_Properties.split pi ((Prims.parse_int "2") * n) with
     | (gamma,cs) ->
         (match FStar_Seq_Properties.split cs n with
          | (c,s) -> ((_OS2ECP gamma), c, s))
-
 let rec _helper_ECVRF_hash_to_curve:
-  Prims.nat -> Prims.nat -> bytes -> bytes -> twisted_edward_point option =
+  Prims.nat -> Prims.nat -> bytes -> bytes -> Spec_Ed25519.ext_point option =
   fun ctr  ->
     fun counter_length  ->
       fun pk  ->
         fun input  ->
           if
             FStar_Option.isNone
-              (_OS2ECP
+              (Spec_Ed25519.point_decompress
                  (hash
                     (seqConcat (seqConcat input pk)
                        (_I2OSP ctr counter_length))))
-          then None
+          then
+            (if (ctr + (Prims.parse_int "1")) < field
+             then
+               _helper_ECVRF_hash_to_curve (ctr + (Prims.parse_int "1"))
+                 counter_length pk input
+             else None)
           else
-            if
-              isPointOnCurve
-                (_OS2ECP
-                   (hash
-                      (seqConcat (seqConcat input pk)
-                         (_I2OSP ctr counter_length))))
-            then
-              _OS2ECP
-                (hash
-                   (seqConcat (seqConcat input pk)
-                      (_I2OSP ctr counter_length)))
-            else
-              if (ctr + (Prims.parse_int "1")) < field
-              then
-                _helper_ECVRF_hash_to_curve (ctr + (Prims.parse_int "1"))
-                  counter_length pk input
-              else None
+            Spec_Ed25519.point_decompress
+              (hash
+                 (seqConcat (seqConcat input pk) (_I2OSP ctr counter_length)))
 let _ECVRF_hash_to_curve:
   bytes -> twisted_edward_point -> twisted_edward_point option =
   fun input  ->
     fun public_key  ->
       _helper_ECVRF_hash_to_curve (Prims.parse_int "0") (Prims.parse_int "4")
         (_ECP2OS public_key) input
-let random: Prims.nat -> Prims.nat =
-  Obj.magic (fun max1  -> failwith "Not yet implemented:random")
+let random: Prims.nat -> Prims.int =
+  fun max1  -> max1 - (Prims.parse_int "1")
 let randBytes: Prims.nat -> bytes =
   fun max1  -> _I2OSP (random max1) (Prims.parse_int "32")
 let _ECVRF_hash_points:
@@ -146,7 +176,7 @@ let _ECVRF_hash_points:
         twisted_edward_point ->
           twisted_edward_point -> twisted_edward_point -> Prims.nat
   =
-  fun generator  ->
+  fun generator1  ->
     fun h  ->
       fun public_key  ->
         fun gamma  ->
@@ -160,206 +190,116 @@ let _ECVRF_hash_points:
                             (seqConcat
                                (seqConcat
                                   (seqConcat
-                                     (seqConcat (_ECP2OS generator)
+                                     (seqConcat (_ECP2OS generator1)
                                         (_ECP2OS h)) (_ECP2OS public_key))
                                   (_ECP2OS gamma)) (_ECP2OS gk)) (_ECP2OS hk)))
                       n))
-let _ECVRF_prove:
-  bytes ->
-    twisted_edward_point -> bytes -> twisted_edward_point -> bytes option
-  =
+let rec little_endian_ins:
+  bytes -> Prims.nat -> bytes -> FStar_UInt8.t FStar_Seq_Base.seq =
+  fun a  ->
+    fun counter  ->
+      fun b  ->
+        if (counter + (Prims.parse_int "1")) < (FStar_Seq_Base.length a)
+        then
+          little_endian_ins a (counter + (Prims.parse_int "1"))
+            (FStar_Seq_Base.upd b
+               (((FStar_Seq_Base.length a) - (Prims.parse_int "1")) - counter)
+               (FStar_Seq_Base.index a counter))
+        else
+          FStar_Seq_Base.upd b
+            (((FStar_Seq_Base.length a) - (Prims.parse_int "1")) - counter)
+            (FStar_Seq_Base.index a counter)
+let little_endian_: bytes -> bytes =
+  fun a  ->
+    little_endian_ins a (Prims.parse_int "0")
+      (FStar_Seq_Base.create (FStar_Seq_Base.length a)
+         (FStar_UInt8.uint_to_t (Prims.parse_int "0")))
+let _ECVRF_prove: bytes -> twisted_edward_point -> bytes -> bytes option =
   fun input  ->
     fun public_key  ->
       fun private_key  ->
-        fun generator  ->
-          if FStar_Option.isNone (_ECVRF_hash_to_curve input public_key)
-          then None
-          else
-            Some
-              (seqConcat
-                 (_ECP2OS
-                    (scalarMultiplication
-                       (FStar_Option.get
-                          (_ECVRF_hash_to_curve input public_key))
-                       private_key))
-                 (seqConcat
-                    (_I2OSP
-                       (_ECVRF_hash_points generator
-                          (FStar_Option.get
-                             (_ECVRF_hash_to_curve input public_key))
-                          public_key
-                          (scalarMultiplication
-                             (FStar_Option.get
-                                (_ECVRF_hash_to_curve input public_key))
-                             private_key)
-                          (scalarMultiplication generator
-                             (_I2OSP (random field) (Prims.parse_int "32")))
-                          (scalarMultiplication
-                             (FStar_Option.get
-                                (_ECVRF_hash_to_curve input public_key))
-                             (_I2OSP (random field) (Prims.parse_int "32"))))
-                       n)
-                    (_I2OSP
-                       (((random field) + field) -
-                          (((_ECVRF_hash_points generator
-                               (FStar_Option.get
-                                  (_ECVRF_hash_to_curve input public_key))
-                               public_key
-                               (scalarMultiplication
-                                  (FStar_Option.get
-                                     (_ECVRF_hash_to_curve input public_key))
-                                  private_key)
-                               (scalarMultiplication generator
-                                  (_I2OSP (random field)
-                                     (Prims.parse_int "32")))
-                               (scalarMultiplication
-                                  (FStar_Option.get
-                                     (_ECVRF_hash_to_curve input public_key))
-                                  (_I2OSP (random field)
-                                     (Prims.parse_int "32"))))
-                              * field)
-                             mod field)) ((Prims.parse_int "2") * n))))
+        if FStar_Option.isNone (_ECVRF_hash_to_curve input public_key)
+        then None
+        else
+          Some
+            (seqConcat
+               (_ECP2OS
+                  (scalarMultiplication
+                     (FStar_Option.get
+                        (_ECVRF_hash_to_curve input public_key))
+                     (little_endian_ private_key)))
+               (seqConcat
+                  (_I2OSP
+                     (_ECVRF_hash_points generator
+                        (FStar_Option.get
+                           (_ECVRF_hash_to_curve input public_key))
+                        public_key
+                        (scalarMultiplication
+                           (FStar_Option.get
+                              (_ECVRF_hash_to_curve input public_key))
+                           (little_endian_ private_key))
+                        (scalarMultiplication generator
+                           (little_endian_
+                              (_I2OSP (random coordinality)
+                                 (Prims.parse_int "32"))))
+                        (scalarMultiplication
+                           (FStar_Option.get
+                              (_ECVRF_hash_to_curve input public_key))
+                           (little_endian_
+                              (_I2OSP (random coordinality)
+                                 (Prims.parse_int "32"))))) n)
+                  (_I2OSP
+                     ((((random coordinality) + coordinality) -
+                         (((_ECVRF_hash_points generator
+                              (FStar_Option.get
+                                 (_ECVRF_hash_to_curve input public_key))
+                              public_key
+                              (scalarMultiplication
+                                 (FStar_Option.get
+                                    (_ECVRF_hash_to_curve input public_key))
+                                 (little_endian_ private_key))
+                              (scalarMultiplication generator
+                                 (little_endian_
+                                    (_I2OSP (random coordinality)
+                                       (Prims.parse_int "32"))))
+                              (scalarMultiplication
+                                 (FStar_Option.get
+                                    (_ECVRF_hash_to_curve input public_key))
+                                 (little_endian_
+                                    (_I2OSP (random coordinality)
+                                       (Prims.parse_int "32")))))
+                             * (_OS2IP private_key))
+                            mod coordinality))
+                        mod coordinality) ((Prims.parse_int "2") * n))))
 let _ECVRF_proof2hash: bytes -> FStar_UInt8.t FStar_Seq_Base.seq =
-  fun pi  -> fst (FStar_Seq_Properties.split pi n)
-let _ECVRF_verify:
-  twisted_edward_point ->
-    twisted_edward_point -> bytes -> bytes -> Prims.bool
-  =
-  fun generator  ->
-    fun public_key  ->
-      fun pi  ->
-        fun input  ->
-          match _ECVRF_decode_proof pi with
-          | (gamma,c,s) ->
-              if Prims.op_Negation (isPointOnCurve gamma)
+  fun pi  ->
+    fst
+      (FStar_Seq_Properties.split
+         (snd (FStar_Seq_Properties.split pi ((Prims.parse_int "2") * n))) n)
+let _ECVRF_verify: twisted_edward_point -> bytes -> bytes -> Prims.bool =
+  fun public_key  ->
+    fun proof  ->
+      fun input  ->
+        match _ECVRF_decode_proof proof with
+        | (gamma,c,s) ->
+            if FStar_Option.isNone gamma
+            then false
+            else
+              if FStar_Option.isNone (_ECVRF_hash_to_curve input public_key)
               then false
               else
-                if FStar_Option.isNone gamma
-                then false
-                else
-                  if
-                    FStar_Option.isNone
-                      (_ECVRF_hash_to_curve input public_key)
-                  then false
-                  else
-                    (_OS2IP c) =
-                      (_ECVRF_hash_points generator
-                         (FStar_Option.get
-                            (_ECVRF_hash_to_curve input public_key))
-                         public_key (FStar_Option.get gamma)
-                         (scalarAddition (scalarMultiplication public_key c)
-                            (scalarMultiplication generator s))
-                         (scalarAddition
-                            (scalarMultiplication (FStar_Option.get gamma) c)
-                            (scalarMultiplication
-                               (FStar_Option.get
-                                  (_ECVRF_hash_to_curve input public_key)) s)))
-
-*)
-
-let one = Prims.parse_int "1"
-let zero = Prims.parse_int "0"    
-
-
-
-let createTwistedEdwardPoint (a: Prims.int)  (b : Prims.int) (c : Prims.int) (d : Prims.int) : Spec_Ed25519.ext_point  =  
-(a,b,c,d)
-
-let printTwistedEdwardPoint (point: Spec_Ed25519.ext_point) = 
-  match point with 
-  | (px, py, pz, pt) -> Printf.printf "point: %s %s %s %s" (to_string px)  (to_string py) (to_string pz) (to_string pt)
-
-
-let testIsPointOnCurve (point: twisted_edward_point) = 
-  let pointOpt = Some point in 
-  let r = isPointOnCurve pointOpt in 
-    printTwistedEdwardPoint point;  Printf.printf " is on the curve? %b" r                                  
-
-
-let printUint8 (a: FStar_UInt8.t)  = 
-  Printf.printf " %s " (FStar_UInt8.to_string a)
-
-
-let printSeqUInt8 (a:  FStar_UInt8.t FStar_Seq_Base.seq) = 
-  let length = FStar_Seq_Base.length a in 
-    let rec print_inside a counter = 
-      if counter < FStar_Seq_Base.length a then 
-        (
-          printUint8 (FStar_Seq_Base.index a counter);
-          print_inside a (counter + one)
-        )
-      else 
-        Printf.printf "\n" 
-    in print_inside a zero  
-
-let createBuffer (length: nat) (value: FStar_UInt8.t) : FStar_UInt8.t FStar_Seq_Base.seq = 
-  FStar_Seq_Base.create (Prims.parse_int (to_string length)) value  
-
-let bufferEqual (a: FStar_UInt8.t FStar_Seq_Base.seq) (b:FStar_UInt8.t FStar_Seq_Base.seq) = 
-  let rec equal_inside a b counter = 
-    if counter < FStar_Seq_Base.length a then 
-        let flag = FStar_UInt8.eq (FStar_Seq_Base.index a counter) (FStar_Seq_Base.index b counter) in 
-          if (flag = false) then false 
-          else equal_inside a b (counter + one)
-    else 
-      true      
-  in (FStar_Seq_Base.length a = FStar_Seq_Base.length b) && equal_inside a b zero    
-                                  
-
-(* test_vectors for _helper_I2OSP*)
-let test_vector1_helper_i2osp : FStar_UInt8.t Prims.list = 
-        [FStar_UInt8.uint_to_t (Prims.parse_int "160"); 
-          FStar_UInt8.uint_to_t (Prims.parse_int "134");
-          FStar_UInt8.uint_to_t (Prims.parse_int "1");]
-
-let test_vector2_helper_i2osp : FStar_UInt8.t Prims.list = 
-        [
-        FStar_UInt8.uint_to_t (Prims.parse_int "160"); 
-        FStar_UInt8.uint_to_t (Prims.parse_int "134"); 
-        FStar_UInt8.uint_to_t (Prims.parse_int "1");
-        FStar_UInt8.uint_to_t (Prims.parse_int "0");
-        FStar_UInt8.uint_to_t (Prims.parse_int "56");
-        FStar_UInt8.uint_to_t (Prims.parse_int "56");
-        FStar_UInt8.uint_to_t (Prims.parse_int "56");
-        ]
-
-let check_helper_i2osp_1 (vector:FStar_UInt8.t Prims.list) =
-      let buffer = createBuffer (Prims.parse_int "3") (FStar_UInt8.of_string "0") in 
-      let result = _helper_I2OSP (Prims.parse_int "100000") buffer (Prims.parse_int "0") in 
-          printSeqUInt8 result;
-      let expected = (FStar_Seq_Properties.createL vector) in 
-          printSeqUInt8 expected;
-          Printf.printf "Test returned %B \n" (bufferEqual expected result);
-     bufferEqual expected result
-
-let check_helper_i2osp_2 (vector:FStar_UInt8.t Prims.list) =
-      let buffer = createBuffer (Prims.parse_int "7") (FStar_UInt8.of_string "0") in 
-      let result = _helper_I2OSP (Prims.parse_int "15824411865220768") buffer (Prims.parse_int "0") in 
-          printSeqUInt8 result;
-      let expected = (FStar_Seq_Properties.createL vector) in 
-          printSeqUInt8 expected;
-          Printf.printf "Test returned %B \n" (bufferEqual expected result);
-     bufferEqual expected result
-
-let check_i2osp_1 (vector:FStar_UInt8.t Prims.list) = 
-    let result = _I2OSP (Prims.parse_int "15824411865220768") (Prims.parse_int "7") in 
-      printSeqUInt8 result;
-    let expected = (FStar_Seq_Properties.createL vector) in
-      printSeqUInt8 expected;
-      Printf.printf "Test returned %B \n" (bufferEqual expected result);
-    bufferEqual expected result
-
-
-let check_osp2i_1 (vector:FStar_UInt8.t Prims.list) = 
-    let vector = (FStar_Seq_Properties.createL vector) in
-    let result = _OS2IP vector in 
-      Printf.printf "The number %s \n" (to_string result);
-      Printf.printf "Test returned %B \n" ((Prims.parse_int "15824411865220768") = result);
-    ((Prims.parse_int "15824411865220768") = result)  
-
-
-let _ = 
-  check_helper_i2osp_1 test_vector1_helper_i2osp;
-  check_helper_i2osp_2 test_vector2_helper_i2osp;
-  check_i2osp_1 test_vector2_helper_i2osp;
-  check_osp2i_1 test_vector2_helper_i2osp                                 
+                (_OS2IP c) =
+                  (_ECVRF_hash_points generator
+                     (FStar_Option.get
+                        (_ECVRF_hash_to_curve input public_key)) public_key
+                     (FStar_Option.get gamma)
+                     (scalarAddition
+                        (scalarMultiplication public_key (little_endian_ c))
+                        (scalarMultiplication generator (little_endian_ s)))
+                     (scalarAddition
+                        (scalarMultiplication (FStar_Option.get gamma)
+                           (little_endian_ c))
+                        (scalarMultiplication
+                           (FStar_Option.get
+                              (_ECVRF_hash_to_curve input public_key))
+                           (little_endian_ s))))
